crypto_proofs/uf1cma/Crypto.Symmetric.UF1CMA.fst
@@ -344,6 +344,45 @@ let modifies_buf_and_ref (#a:Type) (#b:Type) (buf:Buffer.buffer a) (ref:referenc
       (frameOf b == rid /\ live h b /\ disjoint b buf
       /\ disjoint_ref_1 b (HS.as_aref ref)) ==> equal h b h' b))
 
+
+(* TODO: begin here *)
+
+(** From the current memory state, returns the word corresponding to a wordB *)
+noextract val sel_word: h:mem -> b:PL.wordB{live h b} -> GTot word
+let sel_word h b = as_seq h b
+
+(** Only used when mac_log is true *)
+private noextract val _read_word: len:u32 -> b:PL.wordB{length b == UInt32.v len} 
+  -> s:Seq.seq UInt8.t -> i:u32{UInt32.v i <= UInt32.v len} -> ST word
+  (requires (fun h -> live h b /\ Seq.slice (sel_word h b) 0 (UInt32.v i) == s))
+  (ensures  (fun h0 s h1 -> h0 == h1 /\ live h1 b /\ s == sel_word h1 b))
+let rec _read_word len b s i =
+  let h = ST.get () in
+  if UInt32.v i = UInt32.v len then
+    begin
+    Seq.lemma_eq_intro s (sel_word h b);
+    s
+    end
+  else
+    begin
+    let x = b.(i) in
+    let s' = FStar.Seq.(s @| Seq.create 1 x) in
+    Seq.lemma_eq_intro s' (Seq.slice (sel_word h b) 0 (UInt32.v i + 1));
+    _read_word len b s' (FStar.UInt32.(i +^ 1ul))
+    end
+
+noextract val read_word: len:u32 -> b:PL.wordB{length b == UInt32.v len} -> ST word
+  (requires (fun h0 -> live h0 b))
+  (ensures (fun h0 r h1 -> h0 == h1 /\ live h1 b /\ r == (sel_word h1 b)))
+let read_word len b =
+  let h = ST.get() in
+  let s0 = Seq.createEmpty #UInt8.t in
+  Seq.lemma_eq_intro s0 (Seq.slice (sel_word h b) 0 0);
+  _read_word len b s0 0ul
+
+(* TODO: end here *)
+
+
 // update [was add]; could add finalize (for POLY1305 when last block < 16).
 val update: #i:id -> st:state i -> acc:accBuffer i -> w:lbuffer 16 ->
   Stack unit
