crypto_proofs/utils/Crypto.Symmetric.Bytes.fst
@@ -55,7 +55,7 @@ let rec print_buffer s i len =
     ()
 
 // TODO: Deprecate?
-val sel_bytes: h:mem -> l:UInt32.t -> buf:lbuffer (v l){Buffer.live h buf}
+noextract val sel_bytes: h:mem -> l:UInt32.t -> buf:lbuffer (v l){Buffer.live h buf}
   -> GTot (lbytes (v l))
 let sel_bytes h l buf = Buffer.as_seq h buf
 
@@ -64,7 +64,7 @@ let sel_bytes h l buf = Buffer.as_seq h buf
 // Should be polymorphic on the integer size
 // This will be leaky (using implicitly the heap)
 // TODO: We should isolate it in a different module, e.g. Buffer.Alloc
-val load_bytes: l:UInt32.t -> buf:lbuffer (v l) -> Stack (lbytes (v l))
+noextract val load_bytes: l:UInt32.t -> buf:lbuffer (v l) -> Stack (lbytes (v l))
   (requires (fun h0 -> Buffer.live h0 buf))
   (ensures  (fun h0 r h1 -> h0 == h1 /\ Buffer.live h0 buf /\
 		         Seq.equal r (sel_bytes h1 l buf)))
@@ -76,7 +76,7 @@ let rec load_bytes l buf =
     let t = load_bytes (l -^ 1ul) (Buffer.sub buf 1ul (l -^ 1ul)) in
     SeqProperties.cons b t
 
-private val store_bytes_aux: len:UInt32.t -> buf:lbuffer (v len)
+noextract private val store_bytes_aux: len:UInt32.t -> buf:lbuffer (v len)
   -> i:UInt32.t{i <=^ len} -> b:lbytes (v len) -> ST unit
   (requires (fun h0 -> Buffer.live h0 buf /\
     Seq.equal (Seq.slice b 0 (v i)) (sel_bytes h0 i (Buffer.sub buf 0ul i))))
@@ -93,7 +93,7 @@ let rec store_bytes_aux len buf i b =
     store_bytes_aux len buf (i +^ 1ul) b
     end
 
-val store_bytes: l:UInt32.t -> buf:lbuffer (v l) -> b:lbytes (v l) -> ST unit
+noextract val store_bytes: l:UInt32.t -> buf:lbuffer (v l) -> b:lbytes (v l) -> ST unit
   (requires (fun h0 -> Buffer.live h0 buf))
   (ensures  (fun h0 r h1 -> Buffer.live h1 buf /\ Buffer.modifies_1 buf h0 h1 /\
     Seq.equal b (sel_bytes h1 l buf)))
@@ -404,7 +404,7 @@ let rec store_big32 len buf n =
     store_big32 len buf' n';
     buf.(len) <- b // updating after the recursive call helps verification
 
-val uint32_bytes: 
+noextract val uint32_bytes: 
   len:UInt32.t {v len <= 4} -> n:UInt32.t {UInt32.v n < pow2 (8 * v len)} -> 
   Tot (b:lbytes (v len) { UInt32.v n == little_endian b}) (decreases (v len))
 let rec uint32_bytes len n = 
@@ -425,7 +425,7 @@ let rec uint32_bytes len n =
     in 
     SeqProperties.cons byte b'
 
-val uint32_be: 
+noextract val uint32_be: 
   len:UInt32.t {v len <= 4} -> n:UInt32.t {UInt32.v n < pow2 (8 * v len)} -> 
   Tot (b:lbytes (v len) { UInt32.v n == big_endian b}) (decreases (v len))
 let rec uint32_be len n = 
